Improved TM proofs: TMSimp does less rewrites, and has less loops. This might break some names that falled out of TMSimp. TMSimp_old has some of the old behaviour, but the generated names for hypothesis can still be of. Most of the time, the numbers increased, but the order of the hypothesis (as witnessed by the numbers) stayed the same, which eases porting a bit.

theories/TM/Compound/TMTac.v
@@ -73,6 +73,7 @@ Ltac TMSimp1 T :=
   subst;
   unfold finType_CS in *;
   try T;
+  repeat
   match goal with
   | [ H : _ ::: _ = [||]  |- _ ] => inv H
   | [ H : [||] = _ ::: _ |- _ ] => inv H
@@ -98,18 +99,17 @@ Ltac TMSimp1 T :=
       destruct H as (ymid&H)
     end
   | [ x : _ * _    |- _ ] => destruct x
-  | _ => idtac
   end.
 
-Ltac TMSimp2 :=
+Ltac TMSimp2_old :=
   match goal with
   | [ H: ?X = _ |- _ ] => rewrite H in *; lock H
   end.
 
-Tactic Notation "TMSimp" tactic(T) :=
-  repeat progress (repeat progress TMSimp1 T; repeat TMSimp2; unlock all).
+Tactic Notation "TMSimp_old" tactic(T) :=
+  repeat progress (repeat progress TMSimp1 T; repeat TMSimp2_old; unlock all).
 
-Tactic Notation "TMSimp" := TMSimp idtac.
+Tactic Notation "TMSimp_old" := TMSimp_old idtac.
 
 
 (** Rewrite [eq]-assumptions, but only in the goal. This is much faster than [TMSimp]. *)
@@ -117,8 +117,53 @@ Ltac TMSimp_goal :=
   repeat multimatch goal with
          | [ H : ?X = _ |- _ ] => rewrite H
          end.
-  
 
+Fixpoint all_vec {X:Type} {n:nat}  {struct n}: (Vector.t X n -> Prop) -> Prop :=
+  match n with
+      0 => fun A => A (@Vector.nil _)
+    | S n => fun A => forall x, all_vec (fun xs => A (x:::xs))
+  end.
+  
+Lemma all_vec_correct {X:Type} {n:nat} (P : Vector.t X n -> Prop):
+  all_vec P -> forall xs, P xs.
+Proof.  
+  revert P. induction n;cbn;intros. now apply Vector.case0.
+  intros. apply Vector.caseS'. intro. now eapply IHn.
+Qed.    
+Tactic Notation "vector_destruct" hyp(tin) :=
+  let rec introT n :=
+      lazymatch n with
+        0 => idtac
+      |  S ?n =>
+        let x := fresh tin in
+        intro x;introT n
+      end 
+  in
+  let tac n :=  revert dependent tin; intros tin; pattern tin; refine (all_vec_correct _ _);
+    cbv [all_vec];introT n;intros;cbn in *
+  in
+    lazymatch type of tin with
+      tapes _ ?n => tac n
+    | Vector.t _ ?n => tac n
+    end.
+  
+Ltac TMSimp2 :=
+  let tac ts n :=
+    lazymatch InitialRing.isnatcst n with
+      true => vector_destruct ts;try clear ts
+    end
+  in
+    lazymatch goal with
+    | [ ts: tapes _ ?n|- _ ] => tac ts n
+    | [ ts: Vector.t _ ?n|- _ ] => tac ts n
+    | [H : @Vector.nil _ = @Vector.nil _ |-_ ] => clear H
+    end.
+
+
+Tactic Notation "TMSimp" tactic(T) :=
+  repeat progress (repeat progress TMSimp1 T; repeat TMSimp2; unlock all).
+
+Tactic Notation "TMSimp" := TMSimp idtac.
 
 
 (** DO NOT USE THE FOLLOWING (deprecated) TACTICS, except in [TM.Compound]! *)
@@ -156,13 +201,13 @@ Tactic Notation "TMSolve" int_or_var(k) :=
 Tactic Notation "TMCrush" tactic(T) :=
   repeat progress
          (
-           TMSimp T;
+           TMSimp_old T;
            try TMBranche
          ).
 
 Tactic Notation "TMCrush" :=
   repeat progress
          (
-           TMSimp;
+           TMSimp_old;
            try TMBranche
          ).
